msl_application/DagBi_Mark.v
@@ -19,20 +19,13 @@ Require Import RamifyCoq.graph.graph_gen.
 Require Import RamifyCoq.graph.dag.
 Require Import RamifyCoq.graph.weak_mark_lemmas.
 Require Import RamifyCoq.msl_application.Graph.
-Require Import RamifyCoq.msl_application.GraphBi.
 Require Import RamifyCoq.msl_application.Graph_Mark.
+Require Import RamifyCoq.msl_application.GraphBi.
 Require Export RamifyCoq.msl_application.GraphBi_Mark.
 Require Import Coq.Logic.Classical.
 Import RamifyCoq.msl_ext.seplog.OconNotation.
 
 Open Scope logic.
-
-Instance MGS: WeakMarkGraph.MarkGraphSetting bool.
-  apply (WeakMarkGraph.Build_MarkGraphSetting bool
-          (eq true)).
-  intros.
-  destruct x; [left | right]; congruence.
-Defined.
 
 Section SpatialGraph_Mark_Bi.
 
@@ -41,47 +34,40 @@ Context {sSGG_Bi: sSpatialGraph_Graph_Bi bool unit}.
 
 Local Coercion Graph_LGraph: Graph >-> LGraph.
 Local Coercion LGraph_SGraph: LGraph >-> SGraph.
-Local Coercion SGraph_PGraph: SGraph >-> PGraph.
 Local Identity Coercion Graph_GeneralGraph: Graph >-> GeneralGraph.
 Local Identity Coercion LGraph_LabeledGraph: LGraph >-> LabeledGraph.
 Local Identity Coercion SGraph_SpatialGraph: SGraph >-> SpatialGraph.
-Local Identity Coercion PGraph_PreGraph: PGraph >-> PreGraph.
+Local Coercion pg_lg: LabeledGraph >-> PreGraph.
 
 Notation Graph := (@Graph pSGG_Bi bool unit).
 
-Lemma dag_unfold: forall (g: Graph) x d l r,
-  sepcon_unique2 (@vertex_at _ _ _ _ _ SGP) ->
+Lemma root_unfold: forall (g: Graph) x d l r,
   vvalid g x ->
   vgamma g x = (d, l, r) ->
-  dag x g = vertex_at x (vgamma g x) * dags' (l :: r :: nil) g.
-Proof.
-  intros.
-  apply dag_unfold; auto.
-  eapply gamma_step_list; eauto.
-Qed.
+  reachable_dag_vertices_at x g = vertex_at x (d, l, r) * reachable_through_dag_vertices_at (l :: r :: nil) g.
+Proof. apply va_reachable_dag_unfold. Qed.
 
-Lemma dag_vgen: forall (g: Graph) x d l r v,
-  sepcon_unique2 (@vertex_at _ _ _ _ _ SGP) ->
+Lemma root_update_unfold: forall (g: Graph) x d l r v,
   vvalid g x ->
   vgamma g x = (d, l, r) ->
-  dag x (spatialgraph_vgen g x v) = vertex_at x v * dags' (l :: r :: nil) g.
-Proof.
-  intros.
-  apply dag_vgen; auto.
-  eapply gamma_step_list; eauto.
-Qed.
+  reachable_dag_vertices_at x (Graph_gen g x v) = vertex_at x (v, l, r) * reachable_through_dag_vertices_at (l :: r :: nil) g.
+Proof. intros. eapply va_reachable_dag_update_unfold; eauto. Qed.
 
+(* TODO: More modularized way to prove these two RamificationPremise? 
+ For example, handling pure facts? *)
 Lemma dag_ramify_left: forall {RamUnit: Type} (g g1: Graph) x l r,
   vvalid g x ->
   vgamma g x = (false, l, r) ->
   mark1 x g g1 ->
-  (dag x g1: pred) |-- dag l g1 *
-   (ALL a: RamUnit * Graph,
-     !! (mark l g1 (snd a)) -->
-     (dag l (snd a) -* dag x (snd a))).
+  @derives pred _
+    (reachable_dag_vertices_at x g1)
+    (reachable_dag_vertices_at l g1 *
+     (ALL a: RamUnit * Graph,
+       !! (mark l g1 (snd a)) -->
+       (reachable_dag_vertices_at l (snd a) -* reachable_dag_vertices_at x (snd a)))).
 Proof.
   intros.
-  unfold dag.
+  unfold reachable_dag_vertices_at.
   normalize.
   pose proof proj1 H1.
   rewrite <- H3 in H2.
@@ -116,14 +102,14 @@ Lemma dag_ramify_right: forall {RamUnit: Type} (g g1 g2: Graph) x l r,
   vgamma g x = (false, l, r) ->
   mark1 x g g1 ->
   mark l g1 g2 ->
-  (dag x g2: pred) |-- dag r g2 *
+  (reachable_dag_vertices_at x g2: pred) |-- reachable_dag_vertices_at r g2 *
    (ALL a: RamUnit * Graph,
      !! (mark r g2 (snd a)) -->
-     (dag r (snd a) -* dag x (snd a))).
+     (reachable_dag_vertices_at r (snd a) -* reachable_dag_vertices_at x (snd a))).
 Proof.
   intros.
   pose proof @graph_ramify_right _ _ RamUnit g g1 g2 x l r H H0 H1 H2.
-  unfold dag.
+  unfold reachable_dag_vertices_at.
   normalize.
   destruct H1 as [? _].
   destruct H2 as [_ ?].
