sample_mark/env_copy_bi.v
@@ -1,0 +1,19 @@
+Require Export RamifyCoq.veric_ext.SeparationLogic.
+Require Export VST.floyd.proofauto.
+Require Export RamifyCoq.floyd_ext.ramification.
+Require Export RamifyCoq.floyd_ext.semax_ram_lemmas.
+Require Export RamifyCoq.floyd_ext.semax_ram_tac.
+Require Export RamifyCoq.floyd_ext.exists_trick.
+Require Export RamifyCoq.floyd_ext.closed_lemmas.
+Require Export RamifyCoq.floyd_ext.comparable.
+Require Export RamifyCoq.floyd_ext.share.
+Require Export RamifyCoq.sample_mark.copy_bi.
+
+Local Open Scope logic.
+
+Instance CompSpecs : compspecs.
+Proof. make_compspecs prog. Defined.
+
+Global Existing Instance CompSpecs.
+
+Definition node_type := Tstruct _Node noattr.
