sample_mark/verif_copy_bi.v
@@ -1,16 +1,16 @@
 Require Import RamifyCoq.lib.Coqlib.
 Require Import RamifyCoq.lib.EquivDec_ext.
 Require Export VST.floyd.proofauto.
-Require Import RamifyCoq.sample_mark.env_mark_bi.
+Require Import RamifyCoq.sample_mark.env_copy_bi.
 Require Import RamifyCoq.graph.graph_model.
 Require Import RamifyCoq.graph.weak_mark_lemmas.
 Require Import RamifyCoq.graph.path_lemmas.
 Require Import RamifyCoq.graph.subgraph2.
 Require Import RamifyCoq.graph.reachable_computable.
 Require Import RamifyCoq.msl_application.Graph.
+Require Import RamifyCoq.msl_application.Graph_Copy.
 Require Import RamifyCoq.msl_application.GraphBi.
-Require Import RamifyCoq.msl_application.Graph_Mark.
-Require Import RamifyCoq.msl_application.DagBi_Mark.
+Require Import RamifyCoq.msl_application.GraphBi_Copy.
 Require Import RamifyCoq.data_structure.spatial_graph_aligned_bi_VST.
 
 Local Open Scope logic.
@@ -22,7 +22,7 @@ Local Identity Coercion LGraph_LabeledGraph: LGraph >-> LabeledGraph.
 Local Identity Coercion SGraph_SpatialGraph: SGraph >-> SpatialGraph.
 Local Coercion pg_lg: LabeledGraph >-> PreGraph.
 
-Notation dag sh x g := (@reachable_dag_vertices_at _ _ _ _ _ _ _ _ _ (@SGP pSGG_VST bool unit (sSGG_VST sh)) _ x g).
+Notation graph sh x g := (@reachable_vertices_at _ _ _ _ _ _ _ _ _ (@SGP pSGG_VST bool unit (sSGG_VST sh)) _ x g).
 Notation Graph := (@Graph pSGG_VST bool unit).
 Existing Instances MGS biGraph maGraph finGraph RGF.
 
@@ -32,12 +32,12 @@ Definition mark_spec :=
   PRE [ _x OF (tptr (Tstruct _Node noattr))]
           PROP  (weak_valid g x)
           LOCAL (temp _x (pointer_val_val x))
-          SEP   (dag sh x g)
+          SEP   (graph sh x g)
   POST [ Tvoid ]
-      EX g': Graph,
+        EX g': Graph,
         PROP (mark x g g')
-        LOCAL()
-        SEP (dag sh x g').
+        LOCAL ()
+        SEP   (graph sh x g').
 
 Definition main_spec :=
  DECLARE _main
@@ -70,7 +70,7 @@ Proof.
   forward_if_tac  (* if (x == 0) *)
     (PROP  (pointer_val_val x <> nullval)
      LOCAL (temp _x (pointer_val_val x))
-     SEP   (dag sh x g)).
+     SEP   (graph sh x g)).
   admit. (* type checking for pointer comparable. *)
   Focus 1. { (* if-then branch *)
     destruct_pointer_val x.
@@ -92,29 +92,34 @@ Proof.
   } Unfocus.
   destruct_pointer_val x. clear H0 H_weak_valid.
 
-  erewrite root_unfold by eauto.
-  normalize.
-  change (vertex_at x (d, l, r)) with
-    (@data_at CompSpecs sh node_type
-       (Vint (Int.repr (if d then 1 else 0)), (pointer_val_val l, pointer_val_val r)) (pointer_val_val x)).
+  localize
+   (PROP  ()
+    LOCAL (temp _x (pointer_val_val x))
+    SEP   (data_at sh node_type (Vint (Int.repr (if d then 1 else 0)), (pointer_val_val l, pointer_val_val r))
+              (pointer_val_val x))).
+  (* localize *)
 
-  forward. (* root_mark = x -> m; *)
+  apply -> ram_seq_assoc. 
+  eapply semax_ram_seq;
+    [ repeat apply eexists_add_stats_cons; constructor
+    | load_tac
+    | abbreviate_semax_ram].
+  (* root_mark = x -> m; *)
 
-  eapply semax_pre with 
-    (PROP  ()
-     LOCAL 
-      (temp _root_mark (Vint (Int.repr (if d then 1 else 0)));
-      temp _x (pointer_val_val x))
-     SEP  (dag sh x g)).
-  Focus 1. {
-    erewrite root_unfold by eauto.
-    entailer!.
+  unlocalize (PROP ()  LOCAL  (temp _root_mark (Vint (Int.repr (if d then 1 else 0))); temp _x (pointer_val_val x))  SEP  (graph sh x g)).
+
+  Grab Existential Variables.
+  Focus 2. {
+    simplify_ramif.
+    apply (@root_stable_ramify _ (sSGG_VST sh) g x _ H_GAMMA_g); auto.
   } Unfocus.
-  
+  (* unlocalize *)
+
+  unfold semax_ram.
   forward_if_tac  (* if (root_mark == 1) *)
     (PROP   (d = false)
       LOCAL (temp _x (pointer_val_val x))
-      SEP   (dag sh x g)).
+      SEP   (graph sh x g)).
   Focus 1. { (* if-then branch *)
     forward. (* return *)
     apply (exp_right g).
@@ -128,34 +133,63 @@ Proof.
     clear - H0; destruct d; congruence.
   } Unfocus.
 
-  erewrite root_unfold by eauto.
   normalize.
-  change (vertex_at x (false, l, r)) with
-    (@data_at CompSpecs sh node_type
-       (Vint (Int.repr 0), (pointer_val_val l, pointer_val_val r)) (pointer_val_val x)).
+  localize
+   (PROP  ()
+    LOCAL (temp _x (pointer_val_val x))
+    SEP   (data_at sh node_type (Vint (Int.repr 0), (pointer_val_val l, pointer_val_val r))
+              (pointer_val_val x))).
+  (* localize *)
 
-  forward. (* l = x -> l; *)
-  forward. (* r = x -> r; *)
-  forward. (* x -> d = 1; *)
+  apply -> ram_seq_assoc. 
+  eapply semax_ram_seq;
+    [ repeat apply eexists_add_stats_cons; constructor
+    | load_tac
+    | abbreviate_semax_ram].
+  (* l = x -> l; *)
 
-  pose proof Graph_gen_true_mark1 g x _ _ H_GAMMA_g gx_vvalid.
-  apply semax_pre with
+  apply -> ram_seq_assoc.
+  eapply semax_ram_seq;
+    [ repeat apply eexists_add_stats_cons; constructor
+    | load_tac
+    | abbreviate_semax_ram].
+  (* r = x -> r; *)
+
+  apply -> ram_seq_assoc.
+  eapply semax_ram_seq;
+    [ repeat apply eexists_add_stats_cons; constructor
+    | store_tac
+    | abbreviate_semax_ram].
+  cbv beta zeta iota delta [replace_nth].
+  change (@field_at CompSpecs sh node_type []
+           (Vint (Int.repr 1), (pointer_val_val l, pointer_val_val r))) with
+         (@data_at CompSpecs sh node_type
+           (Vint (Int.repr 1), (pointer_val_val l, pointer_val_val r))).
+  (* x -> d = 1; *)
+
+  unlocalize
    (PROP  ()
     LOCAL (temp _r (pointer_val_val r);
            temp _l (pointer_val_val l);
            temp _x (pointer_val_val x))
-    SEP (dag sh x (Graph_gen g x true))).
-  Focus 1. {
-    erewrite root_update_unfold by eauto.
-    entailer!.
+    SEP (graph sh x (Graph_gen g x true))).
+  Grab Existential Variables.
+  Focus 2. {
+    simplify_ramif.
+    apply (@root_update_ramify _ (sSGG_VST sh) g x _ (false, l, r) (true, l, r)); auto.
+    eapply Graph_gen_vgamma; eauto.
   } Unfocus.
+  (* unlocalize *)
 
+  unfold semax_ram. (* should not need this *)
+
+  pose proof Graph_gen_true_mark1 g x _ _ H_GAMMA_g gx_vvalid.
   forget (Graph_gen g x true) as g1.
 
   localize
    (PROP  (weak_valid g1 l)
     LOCAL (temp _l (pointer_val_val l))
-    SEP   (dag sh l g1)).
+    SEP   (graph sh l g1)).
   1: eapply left_weak_valid; eauto.  
   (* localize *)
 
@@ -164,21 +198,21 @@ Proof.
   [ repeat apply eexists_add_stats_cons; constructor
   | semax_ram_call_body (sh, g1, l) 
   | semax_ram_after_call; intros g2;
-    repeat (apply ram_extract_PROP; intro)].
+    repeat (apply ram_extract_PROP; intro) ].
 
   unlocalize
    (PROP  ()
     LOCAL (temp _r (pointer_val_val r);
            temp _l (pointer_val_val l);
            temp _x (pointer_val_val x))
-    SEP (dag sh x g2))
+    SEP (graph sh x g2))
   using [H3]%RamAssu
   binding [g2]%RamBind.
   Grab Existential Variables.
   Focus 2. {
     simplify_ramif.
     subst.
-    eapply (@dag_ramify_left _ (sSGG_VST sh) _ g); eauto.
+    eapply (@graph_ramify_left _ (sSGG_VST sh) _ g); eauto.
   } Unfocus.
   (* unlocalize *)
 
@@ -186,7 +220,7 @@ Proof.
   localize
    (PROP  (weak_valid g2 r)
     LOCAL (temp _r (pointer_val_val r))
-    SEP   (dag sh r g2)).
+    SEP   (graph sh r g2)).
   1: eapply right_weak_valid; eauto.  
   (* localize *)
   
@@ -202,14 +236,14 @@ Proof.
     LOCAL (temp _r (pointer_val_val r);
            temp _l (pointer_val_val l);
            temp _x (pointer_val_val x))
-    SEP (dag sh x g3))
+    SEP (graph sh x g3))
   using [H5]%RamAssu
   binding [g3]%RamBind.
   Grab Existential Variables.
   Focus 2. {
     simplify_ramif.
     subst.
-    eapply (@dag_ramify_right _ (sSGG_VST sh) _ g); eauto.
+    eapply (@graph_ramify_right _ (sSGG_VST sh) _ g); eauto.
   } Unfocus.
   (* Unlocalize *)
 
@@ -218,4 +252,3 @@ Proof.
   apply (exp_right g3); entailer!; auto.
   apply (mark1_mark_left_mark_right g g1 g2 g3 (ValidPointer b i) l r); auto.
 Time Qed. (* Takes 3 hours. *)
-
